とりあえずとばす

full-simpl/chap11.v
@@ -80,110 +80,35 @@ Fixpoint getbinding (n : nat) (ctx: context) :=
     end
   end.
 
-Fixpoint shift (c : nat) (t : term) : term :=
+Fixpoint shift (d k : nat) (t : term) : term :=
 match t with
-| var x => var (if leb c x then (S x) else x)
-| abs x T t' => abs x T (shift (S c) t')
-| app t1 t2 => app (shift c t1) (shift c t2)
+| var x => var (if leb d x then x + k else x)
+| abs x T t' => abs x T (shift (S d) k t')
+| app t1 t2 => app (shift d k t1) (shift d k t2)
 | tru => tru
 | fls => fls
-| If t1 t2 t3 => If (shift c t1) (shift c t2) (shift c t3)
+| If t1 t2 t3 =>
+  If (shift d k t1) (shift d k t2) (shift d k t3)
 | unit => unit
-| seq t1 t2 => seq (shift c t1) (shift c t2)
-end.
-
-Fixpoint unshift (c : nat) (t : term) : term :=
-match t with
-| var x => var (if leb c x then (pred x) else x)
-| abs x T t' => abs x T (unshift (S c) t')
-| app t1 t2 => app (unshift c t1) (unshift c t2)
-| tru => tru
-| fls => fls
-| If t1 t2 t3 => If (unshift c t1) (unshift c t2) (unshift c t3)
-| unit => unit
-| seq t1 t2 => seq (unshift c t1) (unshift c t2)
+| seq t1 t2 =>
+  seq (shift d k t1) (shift d k t2)
 end.
 
 Fixpoint subst (d : nat) (s t: term) : term :=
 match t with
 | var x =>
   if eqb_nat d x then s
-  else t
-| abs x T t' => abs x T (subst (S d) s t')
+  else if ltb d x then var (pred x) else var x
+| abs x T t' => abs x T (subst (S d) (shift 0 1 s) t')
 | app t1 t2 => app (subst d s t1) (subst d s t2)
+| tru => tru
+| fls => fls
+| unit => unit
 | If t1 t2 t3 =>
   If (subst d s t1) (subst d s t2) (subst d s t3)
 | seq t1 t2 =>
   seq (subst d s t1) (subst d s t2)
-| _ => t
 end.
-
-Fixpoint shift_S (d k : nat) (t : term) : term :=
-match t with
-| var x => var (if leb d x then x + k else x)
-| abs x T t' => abs x T (shift_S (S d) k t')
-| app t1 t2 => app (shift_S d k t1) (shift_S d k t2)
-| tru => tru
-| fls => fls
-| If t1 t2 t3 =>
-  If (shift_S d k t1) (shift_S d k t2) (shift_S d k t3)
-| unit => unit
-| seq t1 t2 =>
-  seq (shift_S d k t1) (shift_S d k t2)
-end.
-
-Lemma PM_shift : forall t n,
-    unshift n (shift n t) = t.
-Proof.
-  induction t; simpl; intros; auto.
-  -
-    destruct (leb n0 n) eqn:IH1.
-    apply le_leb in IH1. apply le_S in IH1. apply leb_le in IH1. rewrite IH1. simpl. reflexivity.
-    rewrite IH1. reflexivity.
-  -
-    rewrite IHt. reflexivity.
-  -
-    rewrite IHt1, IHt2; reflexivity.
-  -
-    rewrite IHt1, IHt2, IHt3; reflexivity.
-  -
-    rewrite IHt1, IHt2; reflexivity.
-Qed.
-
-Fixpoint subst_s (d : nat) (s t: term) : term :=
-match t with
-| var x =>
-  if eqb_nat d x then
-    s
-  else
-    if ltb d x then
-      var (pred x) else var x
-| abs x T t' => abs x T (subst_s (S d) s t')
-| app t1 t2 => app (subst_s d s t1) (subst_s d s t2)
-| tru => tru
-| fls => fls
-| unit => unit
-| If t1 t2 t3 =>
-  If (subst_s d s t1) (subst_s d s t2) (subst_s d s t3)
-| seq t1 t2 =>
-  seq (subst_s d s t1) (subst_s d s t2)
-end.
-
-Lemma sub_S : forall t1 t2 n,
-unshift n (subst n (shift n t2) t1) = subst_s n t2 t1.
-Proof.
-  induction t1; simpl; intros; auto.
-  destruct eqb_nat eqn:H. rewrite PM_shift. reflexivity.
-  simpl. destruct ltb eqn:IH1. apply ltb_to_leb in IH1. rewrite IH1. reflexivity.
-  destruct leb eqn:IH2. apply leb_neq_lt in IH2; auto. rewrite IH1 in IH2. inversion IH2.
-  reflexivity.
-
-  rewrite <- IHt1. admit.
-  rewrite IHt1_1, IHt1_2; reflexivity.
-  rewrite IHt1_1, IHt1_2, IHt1_3; reflexivity.
-  rewrite IHt1_1, IHt1_2; reflexivity.
-Abort.
-
 
 Reserved Notation " t '-->i' t' " (at level 40).
 Inductive internal_step :term -> term -> Prop :=
@@ -203,7 +128,7 @@ Inductive internal_step :term -> term -> Prop :=
     app v1 t2 -->i app v1 t2'
 | Ei_AppAbs : forall typ str t12 t2,
     value t2 ->
-    app (abs str typ t12) t2 -->i unshift 0 (subst 0 (shift 0 t2) t12)
+    app (abs str typ t12) t2 -->i subst 0 t2 t12
 
 where " t '-->i' t' " := (internal_step t t').
 
@@ -225,7 +150,7 @@ Inductive external_step : term -> term -> Prop :=
     app v1 t2 -->e app v1 t2'
 | E_AppAbs : forall typ str t12 t2,
     value t2 ->
-    app (abs str typ t12) t2 -->e unshift 0 (subst 0 (shift 0 t2) t12)
+    app (abs str typ t12) t2 -->e subst 0 t2 t12
 | E_seq : forall t1 t1' t2,
     t1 -->e t1' ->
     seq t1 t2 -->e seq t1' t2
@@ -234,86 +159,127 @@ Inductive external_step : term -> term -> Prop :=
     seq v1 t2 -->e t2
 where " t '-->e' t' " := (external_step t t').
 
+Lemma leb_S_l : forall m n,
+  leb (n + S m) n = false.
+Proof.
+  induction n; simpl; intros; auto.
+  destruct eqb_nat eqn:IH1. apply eqb_eq in IH1. rewrite IH1 in IHn. rewrite leb_refl in IHn; inversion IHn.
+  apply leb_F in IHn. apply Nat.nle_gt in IHn. apply Nat.lt_lt_succ_r in IHn. apply lt_not_le in IHn.
+  apply leb_F in IHn. rewrite IHn; reflexivity.
+Qed.
 
-Lemma shift_sub : forall t1 t2 n,
-unshift n (subst n (shift n t2) (shift n t1)) = t1.
+Lemma shift_sub : forall t1 t2 n m,
+    subst n t2 (shift n (S m) t1) = shift n m t1.
 Proof.
   induction t1; intros; simpl; auto.
-  destruct leb eqn:IH1. destruct eqb_nat eqn:IH2. apply eqb_eq in IH2. subst.
-  generalize Nat.nle_succ_diag_l. intros. apply le_leb in IH1. specialize (H n). induction H. apply IH1.
-  simpl. rewrite IH2. rewrite IH1. reflexivity.
-  destruct eqb_nat eqn:IH2. apply eqb_eq in IH2. subst. rewrite leb_refl in IH1. inversion IH1.
-  simpl. rewrite IH1. reflexivity.
-  (* rewrite IHt1. reflexivity. *)
-  admit.
-  rewrite IHt1_1; rewrite IHt1_2; reflexivity.
-  rewrite IHt1_1, IHt1_2, IHt1_3; reflexivity.
-  rewrite IHt1_1, IHt1_2. reflexivity.
-Abort.
-
-Fixpoint e2t t :=
-  match t with
-  | var x => var x
-  | abs x T t' => abs x T (e2t t')
-  | app t1 t2 => app (e2t t1) (e2t t2)
-  | If t1 t2 t3 => If (e2t t1) (e2t t2) (e2t t3)
-  | seq t1 t2 => app (abs "x" Unit (shift 0 (e2t t2))) (e2t t1)
-  | _ => t
-  end.
-
-Lemma shift_sub_1 : forall t1 t2 n,
-    unshift n (subst n (shift 0 t2) (shift n t1)) = t1.
-Proof.
-  induction t1; simpl; intros; auto.
-  destruct (leb n0 n) eqn:IH1.
-  destruct eqb_nat eqn:IH2. apply eqb_eq in IH2. subst.
-  generalize Nat.nle_succ_diag_l; intros. specialize (H n). apply leb_F in H.
-  rewrite H in IH1; inversion IH1.
-  simpl. rewrite IH2. rewrite IH1. reflexivity.
-  destruct eqb_nat eqn:IH2. apply eqb_eq in IH2; subst.
+  destruct leb eqn:IH1; destruct eqb_nat eqn:IH2; try apply eqb_eq in IH2; subst.
+  rewrite leb_S_l in IH1. inversion IH1.
+  apply le_leb in IH1. eapply le_plus_trans with (p:= (S m)) in IH1. apply leb_le in IH1. apply leb_neq_lt in IH1; auto. rewrite IH1. rewrite Nat.add_succ_r. simpl. reflexivity.
   rewrite leb_refl in IH1; inversion IH1.
-  simpl. rewrite IH1. reflexivity.
-
+  destruct ltb eqn:IH3. apply ltb_to_leb in IH3. rewrite IH3 in IH1; inversion IH1.
+  reflexivity.
   rewrite IHt1. reflexivity.
   rewrite IHt1_1, IHt1_2; reflexivity.
   rewrite IHt1_1, IHt1_2, IHt1_3; reflexivity.
   rewrite IHt1_1, IHt1_2; reflexivity.
 Qed.
 
-Lemma subsub : forall t1 t2 n,
-    e2t (subst n t2 t1) = subst n (e2t t2) (e2t t1).
-Proof.
-  induction t1; simpl; intros; auto.
-
-  destruct eqb_nat; auto.
-  rewrite IHt1; reflexivity.
-  rewrite IHt1_1, IHt1_2; reflexivity.
-  rewrite IHt1_1, IHt1_2, IHt1_3; reflexivity.
-  rewrite IHt1_1, IHt1_2.
-
-
-
-Lemma dekinai : forall t n,
-    shift 0 (shift n t) = shift (S n) (shift 0 t).
+Lemma shift_0_t : forall t n,
+    shift n 0 t = t.
 Proof.
   induction t; simpl; intros; auto.
-  repeat rewrite leb0.
-  admit.
-Abort.
+  rewrite <- plus_n_O. destruct leb; reflexivity.
+  rewrite IHt; reflexivity.
+  rewrite IHt1, IHt2; reflexivity.
+  rewrite IHt1, IHt2, IHt3; reflexivity.
+  rewrite IHt1, IHt2; reflexivity.
+Qed.
 
-Lemma shift_e2t : forall t n,
-    e2t (shift n t) = shift n (e2t t).
+Lemma shift_sub_1 : forall t1 t2 n,
+    subst n t2 (shift n 1 t1) = t1.
+Proof.
+  intros. rewrite shift_sub. rewrite shift_0_t. reflexivity.
+Qed.
+
+Fixpoint e t :=
+  match t with
+  | var x => var x
+  | abs x T t' => abs x T (e t')
+  | app t1 t2 => app (e t1) (e t2)
+  | If t1 t2 t3 => If (e t1) (e t2) (e t3)
+  | seq t1 t2 => app (abs "x" Unit (shift 0 1 (e t2))) (e t1)
+  | _ => t
+  end.
+
+Lemma shift_shift : forall t n d1 d2,
+    shift n d1 (shift n d2 t) = shift n (d2 + d1) t.
+Proof.
+  induction t; simpl; intros; auto.
+  -
+    destruct (leb n0 n) eqn:IH1.
+    apply le_leb in IH1. eapply le_plus_trans with (p:= d2) in IH1.
+    apply leb_le in IH1. rewrite IH1. rewrite Nat.add_assoc. reflexivity.
+    rewrite IH1. reflexivity.
+  -
+    rewrite IHt. reflexivity.
+  -
+    rewrite IHt1, IHt2. reflexivity.
+  -
+    rewrite IHt1, IHt2, IHt3; reflexivity.
+  -
+    rewrite IHt1, IHt2; reflexivity.
+Qed.
+
+Lemma leb_S_n_S : forall n m,
+    leb n m = leb (S n) (S m).
+Proof.
+  intros. destruct leb eqn:IH.
+  apply le_leb in IH. apply le_n_S in IH. apply leb_le in IH.
+  rewrite IH. reflexivity.
+  apply leb_F in IH. apply Nat.nle_gt in IH. apply lt_n_S in IH.
+  apply Nat.nle_gt in IH. apply leb_F in IH. rewrite IH; reflexivity.
+Qed.
+
+
+Notation "t1 ';' t2" := (seq t1 t2) (at level 50).
+Notation "'[' n ':=' t2 ']' t1" := (subst n t2 t1) (at level 100).
+
+Fixpoint e2t n t :=
+  match t with
+  | var x => var x
+  | abs x T t' => abs x T (e2t (S n) t')
+  | app t1 t2 => app (e2t n t1) (e2t n t2)
+  | If t1 t2 t3 => If (e2t n t1) (e2t n t2) (e2t n t3)
+  | seq t1 t2 => app (abs "x" Unit (shift n 1 (e2t n t2))) (e2t n t1)
+  | _ => t
+  end.
+
+Lemma shift_e : forall t n1 n2,
+  e2t (S n1) (shift n2 1 t) = shift n2 1 (e2t n1 t) .
 Proof.
   induction t; simpl; intros; auto.
   rewrite IHt. reflexivity.
   rewrite IHt1, IHt2; reflexivity.
   rewrite IHt1, IHt2, IHt3; reflexivity.
-  rewrite IHt1. rewrite IHt2.
-Abort.
+  rewrite IHt1, IHt2.
+Admitted.
 
-Theorem T11_3_1_1_1 : forall t t',
+Lemma subst_e2t : forall t1 t2 n,
+    e2t n ([n := t2]t1) = ([n := (e2t n t2)](e2t (S n) t1)).
+Proof.
+  induction t1; simpl; intros; eauto.
+  destruct eqb_nat; eauto.
+  destruct ltb; auto.
+  rewrite IHt1.
+  rewrite shift_e. reflexivity.
+  rewrite IHt1_1, IHt1_2; reflexivity.
+  rewrite IHt1_1, IHt1_2, IHt1_3; reflexivity.
+  rewrite IHt1_1, IHt1_2.
+Admitted.
+
+Theorem T11_3_1_1_1__ : forall t t',
   t -->e t' ->
-  (e2t t) -->i (e2t t').
+  (e2t 0 t) -->i (e2t 0 t').
 Proof.
   induction t; intros; simpl; try solve_by_inverts 2.
   -
@@ -321,7 +287,8 @@ Proof.
     +
       destruct t1; try solve_by_invert; constructor.
     +
-      admit.
+      rewrite subst_e2t; auto. constructor.
+      destruct t2; try solve_by_invert; constructor.
   -
     inversion H; subst; simpl; try constructor; auto.
   -
@@ -329,15 +296,45 @@ Proof.
     +
       constructor.
     +
-      remember (shift 0 (e2t t')) as s.
-      rewrite <- (shift_sub_1 (e2t t') (e2t t1) 0).
-      subst.
-      constructor. destruct t1; try solve_by_invert; constructor.
+      erewrite <- shift_sub_1.  constructor. destruct t1; try solve_by_invert; constructor.
+Qed.
+
+Lemma subst_e : forall t1 t2 n,
+    e (subst n t2 t1) = subst n (e t2) (e t1).
+Proof.
+  induction t1; intros; simpl; auto; try solve_by_invert.
+  destruct eqb_nat; auto.
+  destruct ltb; auto.
+  rewrite IHt1. admit.
+  rewrite IHt1_1, IHt1_2; reflexivity.
+  rewrite IHt1_1, IHt1_2, IHt1_3; reflexivity.
+  rewrite IHt1_1, IHt1_2.
+Admitted.
+
+Theorem T11_3_1_1_1 : forall t t',
+  t -->e t' ->
+  (e t) -->i (e t').
+Proof.
+  induction t; intros; simpl; try solve_by_inverts 2.
+  -
+    inversion H; subst; simpl; try constructor; auto.
+    +
+      destruct t1; try solve_by_invert; constructor.
+    +
+      rewrite subst_e; auto. constructor; destruct t2; try solve_by_invert; constructor.
+  -
+    inversion H; subst; simpl; try constructor; auto.
+  -
+    inversion H; subst; simpl; try constructor; auto; try solve_by_invert.
+    +
+      constructor.
+    +
+      erewrite <- shift_sub_1. constructor. destruct t1; try solve_by_invert; constructor.
 Qed.
 
 Theorem T11_3_1_1_2 : forall t u,
-  (e2t t) -->i u ->
-  exists t', u = e2t t' /\ t -->e t'.
+  (e t) -->i u ->
+  exists t', u = e t' /\ t -->e t'.
 Proof.
   induction t; simpl; intros; try solve_by_invert.
   -
@@ -349,8 +346,9 @@ Proof.
       destruct t1; try solve_by_invert; constructor.
     +
       destruct t1; try solve_by_invert. simpl in H0. inversion H0; subst.
-      exists (subst 0 t2 t1). split. symmetry. rewrite sub_e2t.
-      constructor. destruct t2; try solve_by_invert; constructor.
+      exists (subst 0 t2 t1). split. symmetry. apply subst_e.
+      constructor.
+      destruct t2; try solve_by_invert; constructor.
   -
     inversion H; subst.
     +
@@ -367,9 +365,8 @@ Proof.
     +
       apply IHt1 in H4. destruct H4; destruct H0; subst. exists (seq x t2); split; try constructor; auto.
     +
-      exists t2. split; try constructor; auto. apply shift_sub. destruct t1; try solve_by_invert; constructor.
+      exists t2. split; try constructor; auto. apply shift_sub_1. destruct t1; try solve_by_invert; constructor.
 Qed.
-
 
 Reserved Notation "ctx '|-' t '\in' T" (at level 40).
 Inductive has_type : context -> term -> ty -> Prop :=
@@ -456,6 +453,24 @@ Proof.
     eapply IHt with (g1:= ((name, typ) :: g1)). apply H5.
 Qed.
 
+Theorem T11_3_1_2 : forall t T ctx n,
+    ctx |- t \in T <->
+    ctx |- (e2t n t) \in T.
+Proof.
+  split; generalize dependent T; generalize dependent ctx; generalize dependent n.
+  -
+    induction t; simpl; intros; auto; inversion H; subst; try solve [econstructor; eauto].
+    +
+      econstructor; eauto. constructor; auto.
+      admit.
+  -
+    induction t; simpl; intros; auto; inversion H; subst; try solve [econstructor; eauto].
+    inversion H3; subst.
+    constructor; eauto. eapply IHt2.
+    admit.
+Abort.
+
+(*
 Theorem T11_3_1_2 : forall t T ctx,
     ctx |- t \in T <->
     ctx |- (e2t t) \in T.
@@ -476,7 +491,7 @@ Proof.
     assert ([] ++ [("x"%string, Unit)] ++ ctx = [("x"%string, Unit)] ++ ctx). reflexivity.
     apply H2.
 Qed.
-
+*)
 End E11_1.
 
 End deBruijin.
@@ -556,29 +571,6 @@ where "t1 '-->' t2" := (step t1 t2).
 
 Definition context := partial_map ty.
 
-Inductive ctx_no : context -> string -> string -> Prop :=
-  | ctx_some : forall ctx x T,
-      ctx x = Some T ->
-      ctx_no ctx x (append x "'")
-  | ctx_none : forall ctx x,
-      ctx x = None ->
-      ctx_no ctx x x.
-
-
-Lemma ctx_no_det : forall x ctx x' x'',
-    ctx_no ctx x x' ->
-    ctx_no ctx x x'' ->
-    ctx x' = None -> ctx x'' = None ->
-    x' = x''.
-Proof.
-  intros. generalize dependent x''.
-  induction H; intros; auto.
-  inversion H0; subst. reflexivity.
-  rewrite H in H2. inversion H2.
-  induction H0; auto.
-  rewrite H in H0. inversion H0.
-Qed.
-
 Inductive appears_free_in : string -> term -> Prop :=
   | afi_var : forall x,
       appears_free_in x (var x)
@@ -608,6 +600,8 @@ Inductive appears_free_in : string -> term -> Prop :=
       appears_free_in x t2 ->
       appears_free_in x (seq t1 t2).
 
+Notation "x '∈fv' t" := (appears_free_in x t) (at level 50).
+
 Fixpoint free x t :=
   match t with
   | var x' => eqb x x'
@@ -625,148 +619,95 @@ Fixpoint free x t :=
     (free x t1) || (free x t2)
   end.
 
-
-Inductive free_name : term -> string -> string -> Prop :=
-  | free_x : forall x t,
-      free x t = true ->
-      free_name t x (append x "'")
-  | not_free : forall x t,
-      free x t = false ->
-      free_name t x x.
-
-Lemma name_det : forall x x1 x2 t,
-    free_name t x x1 ->
-    free_name t x x2 ->
-    x1 = x2.
-Proof.
-  intros. generalize dependent x2; induction H; intros;
-  induction H0; auto; rewrite H in H0; inversion H0.
-Qed.
-
-Inductive multi_name : term -> string -> string -> Prop :=
-| name_refl : forall x t,
-    multi_name t x x
-| name_malti : forall t x1 x2 x3,
-    free_name t x1 x2 ->
-    free_name t x2 x3 ->
-    multi_name t x1 x3.
-
-Lemma multi_det : forall t x x1 x2,
-    multi_name t x x1 -> multi_name t x x2 ->
-    free x1 t = false -> free x2 t = false ->
-    x1 = x2.
-Proof.
-  intros. generalize dependent x2. induction H; intros.
-  inversion H0; subst; auto.
-  admit.
-  admit.
-Admitted.
-
-
-Inductive e2t : term -> context -> term -> Prop :=
-| evar : forall x ctx, e2t (var x) ctx (var x)
-| eabs : forall x T t t' ctx,
-    e2t t ctx t' ->
-    e2t (abs x T t) ctx (abs x T t')
-| eapp : forall t1 t2 t1' t2' ctx,
-    e2t t1 ctx t1' -> e2t t2 ctx t2' ->
-    e2t (app t1 t2) ctx (app t1' t2')
-| etru : forall ctx,
-    e2t tru ctx tru
-| efls : forall ctx,
-    e2t fls ctx fls
-| eunit : forall ctx,
-    e2t unit ctx unit
-| eif : forall ctx t1 t2 t3 t1' t2' t3',
-    e2t t1 ctx t1' -> e2t t2 ctx t2' -> e2t t3 ctx t3' ->
-    e2t (If t1 t2 t3) ctx (If t1' t2' t3')
-| eseq : forall x ctx t1 t2 t1' t2',
-    free_name (seq t1 t2) "x" x ->
-    e2t t1 ctx t1' -> e2t t2 ctx t2' ->
-    e2t (seq t1 t2) ctx (app (abs x Unit t2') t1').
-
-Lemma e2t_det : forall t t1 t2 ctx1 ctx2,
-    e2t t ctx1 t1 ->
-    e2t t ctx2 t2 ->
-    t1 = t2.
-Proof.
-  induction t; simpl; intros; inversion H; inversion H0; subst; auto .
-  erewrite IHt with (t1:= t'); eauto.
-  erewrite IHt1 with (t2:= t1'); eauto. erewrite IHt2 with (t1:= t2'); eauto.
-  erewrite IHt1 with (t2:= t1'); eauto. erewrite IHt2 with (t1:= t2'); eauto. erewrite IHt3 with (t1:= t3'); eauto.
-  erewrite IHt2 with (t1:= t2'); eauto. erewrite IHt1 with (t2:= t1'); eauto.
-  erewrite name_det with (x1:= x); eauto.
-Qed.
-
-Lemma sub_E : forall t12 t2 n ctx t2' t12',
-    e2t t2 ctx t2' -> e2t t12 ctx t12' ->
-    e2t (subst n t2 t12) ctx (subst n t2' t12').
-Proof.
-  induction t12; simpl; intros; inversion H0; subst; simpl; eauto; try solve [inversion H1; subst; auto].
-  destruct eqb; auto.
-  destruct eqb; eauto. apply eabs; auto.
-  apply eapp; auto.
-  apply eif; auto.
-  destruct eqb; auto.
-  admit.
-
-  inversion H0; subst.
-  apply eseq; auto.
-  destruct (free "x" (seq ([n := t2] t12_1) ([n:= t2] t12_2) )) eqn:IH.
-
-Admitted.
-
-Theorem T11_3_1_1 : forall t t' ctx t1 t1',
-  t --> t' ->
-  e2t t ctx t1 -> e2t t' ctx t1' ->
-  t1 --> t1'.
-Proof.
-  intros. generalize dependent t1; generalize dependent t1'.
-  induction H; intros.
-
-  -
-    inversion H0; subst. inversion H4; subst.
-    eapply sub_E with (n:= x) in H7; eauto. eapply e2t_det with (t2:= t1') in H7; eauto. subst. apply E_AppAbs.
-
-
-
-  induction t; intros; try solve_by_invert.
-  -
-    inversion H0; subst. inversion H; subst.
-    inversion H4; subst. eapply sub_E with (n:= x) in H1; eauto. erewrite e2t_det with (t:= ()). apply E_AppAbs; auto.
-    inversion H6; subst; destruct t2'; try solve_by_invert; constructor.
-
-    inversion H1; subst. eapply e2t_det in H7; eauto; subst. apply E_App1; auto.
-    eapply IHt1; eauto.
-
-    inversion H1; subst.
-    eapply e2t_det in H4; eauto; subst. apply E_App2; auto.
-    inversion H5; subst; inversion H6; subst; constructor.
-    eapply IHt2; eauto.
-  -
-    inversion H0; subst. inversion H; subst.
-    inversion H5; subst. eapply e2t_det in H1; eauto; subst; constructor.
-    inversion H5; subst. eapply e2t_det in H1; eauto; subst; constructor.
-
-    inversion H1; subst. eapply e2t_det in H8; eauto; subst. eapply e2t_det in H9; eauto; subst.
-    apply E_If. eapply IHt1; eauto.
-  -
-    inversion H0; subst.
-    eapply e2t_det in H5; eauto; subst.
-    eapply name_det in H4; eauto; subst. eapply e2t_det in H8; eauto; subst. apply E_App2.
-    constructor. eapply IHt1; eauto.
-
-    eapply e2t_det in H1; eauto; subst.
-    rewrite <- (value_subst t1' t1'0 x).
-    assert (abs x Unit ([x := t1'0]t1') = abs x Unit t1').
-    rewrite (value_subst t1' t1'0 x). reflexivity.
-    admit.
-    rewrite H1.
-    apply E_AppAbs. inversion H8; subst; inversion H6; subst; constructor.
-    admit.
-Admitted.
+Fixpoint e x t :=
+  match t with
+  | abs s T t' => abs s T (e x t')
+  | app t1 t2 => app (e x t1) (e x t2)
+  | If t1 t2 t3 => If (e x t1) (e x t2) (e x t3)
+  | seq t1 t2 => app (abs x Unit (e x t2)) (e x t1)
+  | _ => t
+  end.
 
 Open Scope string.
+Lemma subst_e_free : forall t1 t2 x,
+    not (x ∈fv t1) ->
+    [x := t2]t1 = t1.
+Proof.
+  induction t1; simpl; intros; auto;
+    try (rewrite IHt1_1, IHt1_2; try rewrite IHt1_3; auto; intro; apply H; solve [constructor; auto]).
+  -
+    destruct eqb eqn:IH; auto. apply String.eqb_eq in IH; subst.
+    induction H. constructor.
+  -
+    destruct eqb eqn:IH; auto. rewrite IHt1; auto.
+    intro. apply H. constructor. intro. subst. rewrite String.eqb_refl in IH.
+    inversion IH. apply H0.
+Qed.
+
+
+Lemma afi_e : forall t x,
+    x ∈fv e x t -> x ∈fv t.
+Proof.
+  induction t; simpl; intros; auto.
+  inversion H; subst. constructor; auto.
+  inversion H; subst; solve [constructor; auto].
+  inversion H; subst; solve [constructor; auto].
+  inversion H; subst; try solve [constructor; auto].
+  inversion H2; subst. solve [constructor; auto].
+Qed.
+
+
+Lemma subst_e : forall t1 t2 x x',
+    not (x' ∈fv t1) ->
+    e x ([x':= t2]t1) = [x' := e x t2](e x t1).
+Proof.
+  induction t1; simpl; intros; auto.
+  destruct eqb; auto.
+  destruct eqb eqn:IH. apply String.eqb_eq in IH; subst; auto.
+  rewrite IHt1; auto.
+  intro. apply H. constructor. intro; subst. rewrite String.eqb_refl in IH. inversion IH. apply H0.
+  rewrite IHt1_1, IHt1_2; auto; intro; apply H; solve [constructor; auto].
+  rewrite IHt1_1, IHt1_2, IHt1_3; auto; intro; apply H; solve [constructor; auto].
+  rewrite IHt1_1, IHt1_2; auto. destruct eqb eqn:IH; auto. apply String.eqb_eq in IH; subst.
+  rewrite subst_e_free. reflexivity.
+  intro. apply H. apply afi_seq2. apply afi_e. apply H0.
+  intro. apply H; solve [constructor; auto].
+  intro. apply H; solve [constructor; auto].
+Qed.
+
+Theorem T11_3_1_1 : forall t t' x,
+  t --> t' ->
+  not (x ∈fv t) -> not (x ∈fv t') ->
+  e x t --> e x t'.
+Proof.
+  induction t; simpl; intros; try solve_by_invert.
+  -
+    inversion H; subst.
+    +
+      rewrite subst_e. constructor; auto. destruct t2; try solve_by_invert; constructor.
+      admit.
+    +
+      constructor. apply IHt1; auto.
+      intro; apply H0; constructor; auto.
+      intro; apply H1; constructor; auto.
+    +
+      constructor; auto. destruct t1; try solve_by_invert; constructor.
+      apply IHt2; auto; intro.
+      apply H0; solve[constructor; auto].
+      apply H1; solve[constructor; auto].
+  -
+    inversion H; subst; simpl; try constructor; auto.
+    apply IHt1; auto; intro. apply H0; constructor; auto.
+    apply H1; solve[constructor; auto].
+  -
+    inversion H; subst; simpl.
+    +
+      constructor; auto. destruct t2; try solve_by_invert; constructor.
+      apply IHt1; auto; intro.
+      apply H0; constructor; auto.
+      apply H1; constructor; auto.
+Admitted.
+
 
 Reserved Notation "ctx '|-' t '\in' T" (at level 40).
 Inductive has_type : context -> term -> ty -> Prop :=
@@ -791,57 +732,6 @@ Inductive has_type : context -> term -> ty -> Prop :=
        ctx |- If t1 t2 t3 \in T
 
 where "ctx '|-' t '\in' T" := (has_type ctx t T).
-
-
-Reserved Notation "ctx '|-e' t '\in' T" (at level 40).
-Inductive ehas_type : context -> Eterm -> ty -> Prop :=
-  | eT_Var : forall ctx x T,
-      ctx x = Some T ->
-      ctx |-e Var x \in T
-  | eT_Abs : forall ctx x T11 T12 t12,
-      (x |-> T11 ; ctx) |-e t12 \in T12 ->
-      ctx |-e Abs x T11 t12 \in Arrow T11 T12
-  | eT_App : forall T11 T12 ctx t1 t2,
-      ctx |-e t1 \in Arrow T11 T12 ->
-      ctx |-e t2 \in T11 ->
-      ctx |-e App t1 t2 \in T12
-  | eT_Tru : forall ctx,
-       ctx |-e Tru \in Bool
-  | eT_Fls : forall ctx,
-       ctx |-e Fls \in Bool
-  | eT_If : forall t1 t2 t3 T ctx,
-       ctx |-e t1 \in Bool ->
-       ctx |-e t2 \in T ->
-       ctx |-e t3 \in T ->
-       ctx |-e EIf t1 t2 t3 \in T
-  | eT_Seq : forall ctx t1 t2 T2,
-      ctx |-e t1 \in Unit ->
-      ctx |-e t2 \in T2 ->
-      ctx |-e seq t1 t2 \in T2
-
-where "ctx '|-e' t '\in' T" := (ehas_type ctx t T).
-
-
-Theorem T11_3_1_2 : forall t ctx t' T,
-    e2t t ctx t' ->
-    ctx |-e t \in T <-> ctx |- t' \in T.
-Proof.
-  split;
-  generalize dependent t'; generalize dependent T; generalize dependent ctx;
-  induction t; intros; inversion H; subst; inversion H0; subst; auto; try solve [constructor; auto].
-
-  eapply T_App; eauto.
-
-  eapply T_App; eauto. apply T_Abs; auto.
-
-
-  generalize dependent t'. generalize dependent T. generalize dependent ctx.
-  induction t; intros; inversion H; subst; inversion H0; subst; auto; try solve [constructor; auto].
-
-  apply eT_Abs; auto. eapply IHt in H7; eauto. admit.
-
-
-
 
 End Seq.
 
